Move everything out of sections

warblreequiv/LWEquivTMatcher.v
@@ -116,425 +116,420 @@ Inductive equiv_results: TMatchResult -> MatchState -> open_groups -> MatchResul
 | Equiv_results_errr: forall t' ms open_gl errr, equiv_results t' ms open_gl (Error errr).
 
 
-Section Main.
-  Context (str0: string).
+(* A continuation is always called at a fixed position in the regexp, so with a fixed list of
+   groups that are currently open.
+   We say that a MatcherContinuation mc and a TMatcherContinuation tmc are equivalent under a given input string str0 and the list of
+   open groups open_gl when given any MatchState ms compatible with the string str0 being matched,
+   the sub-backtree (tmc s) with extended match state (s, open_gl) is equivalent to the MatchResult
+   (mc s). *)
+Definition equiv_tree_mcont (str0: string) (mc: MatcherContinuation) (tmc: TMatcherContinuation) (gl: open_groups) :=
+  forall s: MatchState,
+  MatchState.input s = str0 -> 
+  equiv_results (tmc s) s gl (mc s).
 
-  (* A continuation is always called at a fixed position in the regexp, so with a fixed list of
-     groups that are currently open.
-     We say that a MatcherContinuation mc and a TMatcherContinuation tmc are equivalent under the list of
-     open groups open_gl when given any MatchState ms compatible with the string str0 being matched,
-     the sub-backtree (tmc s) with extended match state (s, open_gl) is equivalent to the MatchResult
-     (mc s). *)
-  Definition equiv_tree_mcont (mc: MatcherContinuation) (tmc: TMatcherContinuation) (gl: open_groups) :=
-    forall s: MatchState,
-    MatchState.input s = str0 -> 
-    equiv_results (tmc s) s gl (mc s).
-
-  (* A (T)Matcher matches a regexp, then calls a continuation after matching the said regexp.
-     We say that a Matcher m and a TMatcher tm are equivalent when given equivalent continuations,
-     we obtain back equivalent continuations. *)
-  Definition equiv_tree_matcher (m: Matcher) (tm: TMatcher) :=
-    forall mc tmc gl, equiv_tree_mcont mc tmc gl -> equiv_tree_mcont (fun s => m s mc) (fun s => tm s tmc) gl.
+(* A (T)Matcher matches a regexp, then calls a continuation after matching the said regexp.
+   We say that a Matcher m and a TMatcher tm are equivalent under the input string str0 when given equivalent continuations,
+   we obtain back equivalent continuations. *)
+Definition equiv_tree_matcher (str0: string) (m: Matcher) (tm: TMatcher) :=
+  forall mc tmc gl, equiv_tree_mcont str0 mc tmc gl -> equiv_tree_mcont str0 (fun s => m s mc) (fun s => tm s tmc) gl.
 
 
-  (* The identity continuations. *)
-  Definition id_mcont: MatcherContinuation := fun x => Success (Some x).
-  Definition id_tmcont: TMatcherContinuation := fun _ => Success Match.
+(* The identity continuations. *)
+Definition id_mcont: MatcherContinuation := fun x => Success (Some x).
+Definition id_tmcont: TMatcherContinuation := fun _ => Success Match.
 
-  (* These two continuations are easily equivalent. *)
-  Lemma id_equiv: equiv_tree_mcont id_mcont id_tmcont nil.
-  Proof.
-    intro s. unfold id_mcont, id_tmcont. constructor. reflexivity.
-  Qed.
+(* These two continuations are easily equivalent (under all input strings and with no groups opened). *)
+Lemma id_equiv: forall str0, equiv_tree_mcont str0 id_mcont id_tmcont nil.
+Proof.
+  constructor. reflexivity.
+Qed.
 
-  Lemma repeatMatcher'_tRepeatMatcher': forall (m: Matcher) (tm: TMatcher),
-    equiv_tree_matcher m tm ->
-    forall fuel: nat,
-    forall (min: non_neg_integer) (max: non_neg_integer_or_inf) (greedy: bool)
-    (parenIndex parenCount: non_neg_integer),
-    equiv_tree_matcher
-      (fun ms mc => Semantics.repeatMatcher' m min max greedy ms mc parenIndex parenCount fuel)
-      (fun ms tmc => tRepeatMatcher' tm min max greedy ms tmc parenIndex parenCount fuel).
-  Proof.
-    intros m tm Hm_tm_equiv fuel.
-    induction fuel as [|fuel IHfuel].
-    - simpl. constructor.
-    - intros min max greedy parenIndex parenCount mc tmc gl Hequivcont x Hxstr0.
-      simpl.
-      destruct (max =? 0)%NoI eqn:Hmax0; simpl.
-      (* Case max = 0: use hypothesis on continuation *)
-      + unfold equiv_tree_mcont in Hequivcont.
-        now apply Hequivcont.
-      (* Case max > 0 *)
-      + (* Assume that the capture reset succeeds *)
-        destruct List.List.Update.Nat.Batch.update as [cap'|] eqn:Heqcap'; simpl. 2: constructor.
-        remember (match_state (MatchState.input x) (MatchState.endIndex x) cap') as s'.
-        remember (fun y: MatchState => _) as tmc'.
-        remember (fun (y: MatchState) => (_: MatchResult)) as mc'.
-        assert (equiv_tree_mcont mc' tmc' gl) as Hequiv'.
-        {
-          intros s Hsstr0.
-          rewrite Heqmc', Heqtmc'.
-          destruct ((min ==? 0)%wt && _) eqn:Hprogress; simpl.
-          - constructor. reflexivity.
-          - remember (if (min ==? 0)%wt then 0 else min - 1) as min'.
-            remember (if (max =? +∞)%NoI then +∞ else (max - 1)%NoI) as max'.
-            specialize (IHfuel min' max' greedy parenIndex parenCount mc tmc gl Hequivcont s Hsstr0).
-            inversion IHfuel.
-            + simpl. constructor. simpl. assumption.
-            + constructor.
-            + constructor.
-        }
-        assert (equiv_results (tm s' tmc') s' gl (m s' mc')) as Hequivres.
-        {
-          unfold equiv_tree_matcher in Hm_tm_equiv.
-          specialize (Hm_tm_equiv mc' tmc' gl Hequiv' s').
-          assert (Hs'str0: MatchState.input s' = str0).
-          {
-            rewrite Heqs'. simpl. assumption.
-          }
-          specialize (Hm_tm_equiv Hs'str0).
-          inversion Hm_tm_equiv.
-          2,3: constructor.
-          now constructor.
-        }
-        assert ((reset_groups_ms (seq (parenIndex + 1) parenCount) x) = s') as RESET_GROUPS.
-        {
-          unfold reset_groups_ms.
-          destruct x.
-          rewrite <- List.List.Range.Nat.Length.range_seq.
-          unfold List.List.Range.Nat.Bounds.range in Heqcap'.
-          rewrite decr_range by lia.
-          replace (parenIndex + parenCount + 1 - 1 - (parenIndex + 1 - 1)) with parenCount in Heqcap' by lia.
-          simpl in Heqcap'.
-          rewrite Heqcap'.
-          simpl in *.
-          congruence.
-        }
-        destruct (negb (min =? 0)) eqn:Hmin_nonzero; simpl.
-        (* Case min > 0 *)
-        * inversion Hequivres.
-          2,3: constructor.
-          constructor. simpl.
-          rewrite RESET_GROUPS.
-          simpl.
-          assumption.
-        (* Case min = 0 *)
-        * specialize (Hequivcont x Hxstr0).
-          inversion Hequivcont; inversion Hequivres; destruct greedy eqn:Hgreedy; simpl.
-          all: try constructor.
-          (* There must be a way to make this simpler *)
-          -- subst ms open_gl ms0 open_gl0.
-              rename t0 into z.
-              rename t into z'.
-              rename res0 into zm.
-              unfold "!=?".
-              destruct (zm ==? None)%wt eqn:Hzm_None; simpl.
-              ++ constructor. simpl. rewrite RESET_GROUPS.
-                (* rewrite H8. simpl. *)
-                rewrite EqDec.inversion_true in Hzm_None.
-                rewrite <- H8.
-                rewrite Hzm_None.
-                assumption.
-              ++ constructor. simpl. rewrite RESET_GROUPS.
-                rewrite <- H8. simpl.
-                rewrite EqDec.inversion_false in Hzm_None.
-                destruct zm; simpl.
-                ** reflexivity.
-                ** contradiction.
-          -- subst ms open_gl ms0 open_gl0.
-              rename t0 into z.
-              rename t into z'.
-              rename res0 into zm.
-              rename res into zmc.
-              unfold "!=?".
-              destruct (zmc ==? None)%wt eqn:Hzmc_None; simpl.
-              ++ constructor. simpl. rewrite <- H3. simpl.
-                rewrite EqDec.inversion_true in Hzmc_None.
-                rewrite Hzmc_None.
-                rewrite RESET_GROUPS.
-                simpl.
-                assumption.
-              ++ constructor. simpl. rewrite <- H3. simpl.
-                rewrite EqDec.inversion_false in Hzmc_None.
-                destruct zmc; simpl.
-                ** reflexivity.
-                ** contradiction.
-
-          -- subst ms open_gl ms0 open_gl0.
-              rewrite <- H4.
-              destruct t'.
-              ++ simpl.
-                unfold "!=?".
-                destruct (res ==? None)%wt eqn:Hres_None; simpl.
-                ** constructor.
-                ** constructor. simpl. rewrite <- H3.
-                    simpl.
-                    rewrite EqDec.inversion_false in Hres_None.
-                    destruct res.
-                    --- reflexivity.
-                    --- contradiction.
-              ++ simpl. constructor.
-          
-          -- subst ms open_gl ms0 open_gl0.
-              rewrite <- H.
-              destruct t'.
-              ++ simpl.
-                unfold "!=?".
-                destruct (res ==? None)%wt eqn:Hres_None; simpl.
-                ** constructor.
-                ** constructor. simpl. rewrite RESET_GROUPS.
-                    rewrite <- H7. simpl.
-                    rewrite EqDec.inversion_false in Hres_None.
-                    now destruct res.
-              ++ simpl. constructor.
-  Qed.
-
-
-  Theorem compile_tcompile: forall reg ctx rer m tm
-    (Heqm: Semantics.compileSubPattern reg ctx rer forward = Success m)
-    (Heqtm: tCompileSubPattern reg ctx rer forward = Success tm),
-    equiv_tree_matcher m tm.
-  Proof.
-    intros reg ctx rer.
-    revert ctx.
-    induction reg as [
-      |
-      chr |
-      |
-      ae |
-      cc |
-      wr1 IH1 wr2 IH2 |
-      wr IH q |
-      wr1 IH1 wr2 IH2 |
-      name wr IH |
-      |
-      |
-      |
-      |
-      wr IH |
-      wr IH |
-      wr IH |
-      wr IH
-    ]; simpl.
-
-    - (* Empty *)
-      intros. inversion Heqm as [Heqm']. inversion Heqtm as [Heqtm'].
-      intros mc tmc gl Hequiv ms Hmsstr0.
-      apply Hequiv. assumption.
-    
-    - (* Character *)
-      intros. unfold equiv_tree_matcher. intros mc tmc gl Hequiv ms Hmsstr0.
-      inversion Heqtm as [Heqtm']. clear Heqtm Heqtm'.
-      inversion Heqm as [Heqm']. clear Heqm Heqm'.
-      unfold tCharacterSetMatcher, Semantics.characterSetMatcher.
-      simpl.
-      remember ((_ <? 0)%Z || _) as oob.
-      destruct oob eqn:Hoob.
-      + constructor. reflexivity.
-      + remember (Z.min _ _) as index.
-        remember (List.List.Indexing.Int.indexing _ _) as readchr.
-        destruct readchr as [readchr|]; simpl. 2: constructor.
-        remember (CharSet.exist_canonicalized _ _ _) as read_matches.
-        destruct read_matches eqn:Hread_matches; simpl.
-        2: constructor; reflexivity.
-        remember (match_state _ _ _) as ms'.
-        specialize (Hequiv ms').
-        assert (MatchState.input ms' = str0) as Hms'str0.
-        {
-          rewrite Heqms'. simpl. apply Hmsstr0.
-        }
-        specialize (Hequiv Hms'str0).
-        destruct (tmc ms') as [child|]; simpl. 2: constructor.
-        destruct (mc ms') as [res|]; simpl. 2: constructor.
-        constructor.
-        replace (Z.min (MatchState.endIndex ms) (MatchState.endIndex ms + 1)) with (MatchState.endIndex ms) in Heqindex by lia.
-        rewrite Heqindex in Heqreadchr.
-        simpl.
-        inversion Hequiv as [child0 ms'0 gl0 res0 Hequiv' Heqchild0 Heqms'0 Heqgl0 Heqres0 | |].
-        unfold advance_ms.
-        rewrite <- Heqms'.
-        rewrite <- Hequiv'.
-        reflexivity.
-    
-    - (* Dot; same as character *)
-      intros. unfold equiv_tree_matcher. intros mc tmc gl Hequiv ms Hmsstr0.
-      inversion Heqtm as [Heqtm']. clear Heqtm Heqtm'.
-      inversion Heqm as [Heqm']. clear Heqm Heqm'.
-      unfold tCharacterSetMatcher, Semantics.characterSetMatcher.
-      simpl.
-      remember ((_ <? 0)%Z || _) as oob.
-      destruct oob eqn:Hoob.
-      + constructor. reflexivity.
-      + remember (Z.min _ _) as index.
-        remember (List.List.Indexing.Int.indexing _ _) as readchr.
-        destruct readchr as [readchr|]; simpl. 2: constructor.
-        remember (CharSet.exist_canonicalized _ _ _) as read_matches.
-        destruct read_matches eqn:Hread_matches; simpl.
-        2: constructor; reflexivity.
-        remember (match_state _ _ _) as ms'.
-        specialize (Hequiv ms').
-        assert (MatchState.input ms' = str0) as Hms'str0.
-        {
-          rewrite Heqms'. simpl. apply Hmsstr0.
-        }
-        specialize (Hequiv Hms'str0).
-        destruct (tmc ms') as [child|]; simpl. 2: constructor.
-        destruct (mc ms') as [res|]; simpl. 2: constructor.
-        constructor.
-        replace (Z.min (MatchState.endIndex ms) (MatchState.endIndex ms + 1)) with (MatchState.endIndex ms) in Heqindex by lia.
-        rewrite Heqindex in Heqreadchr.
-        simpl.
-        inversion Hequiv as [child0 ms'0 gl0 res0 Hequiv' Heqchild0 Heqms'0 Heqgl0 Heqres0 | |].
-        unfold advance_ms.
-        rewrite <- Heqms'.
-        rewrite <- Hequiv'.
-        reflexivity.
-    
-    - (* Atom escape: unsupported *)
-      intros. destruct (match ae with | DecimalEsc de => _ | ACharacterClassEsc cce => _ | ACharacterEsc ce => _ | GroupEsc gn => _ end); discriminate.
-    
-    - (* Character class: unsupported *)
-      intros. destruct (let! _ =<< _ in _); discriminate.
-    
-    - (* Disjunction *)
-      intros.
-      remember (Disjunction_left wr2 :: ctx) as ctxleft.
-      remember (Disjunction_right wr1 :: ctx) as ctxright.
-      specialize (IH1 ctxleft).
-      specialize (IH2 ctxright).
-      destruct (Semantics.compileSubPattern wr1 _ _ _) as [m1|] eqn:Heqm1; simpl. 2: discriminate.
-      destruct (Semantics.compileSubPattern wr2 _ _ _) as [m2|] eqn:Heqm2; simpl. 2: discriminate.
-      destruct (tCompileSubPattern wr1 _ _ _) as [tm1|] eqn:Heqtm1; simpl. 2: discriminate.
-      destruct (tCompileSubPattern wr2 _ _ _) as [tm2|] eqn:Heqtm2; simpl. 2: discriminate.
-      simpl in *.
-      unfold equiv_tree_matcher.
-      intros mc tmc gl Hequiv ms' Hms'str0.
-      specialize (IH1 m1 tm1 eq_refl eq_refl mc tmc gl Hequiv ms' Hms'str0).
-      specialize (IH2 m2 tm2 eq_refl eq_refl mc tmc gl Hequiv ms' Hms'str0).
-      simpl in *.
-      inversion Heqtm as [Heqtm'].
-      destruct (tm1 ms' tmc) as [t1|] eqn:Heqt1; simpl. 2: constructor.
-      destruct (tm2 ms' tmc) as [t2|] eqn:Heqt2; simpl. 2: constructor.
-      inversion Heqm as [Heqm'].
-      destruct (m1 ms' mc) as [r|] eqn:Heqr; simpl. 2: constructor.
-      destruct r eqn:?; simpl.
-      + constructor. inversion IH1 as [t1' ms'' gl' res IH1' Heqt1' Heqms'' Heqgl' Heqres | |].
-        simpl. rewrite <- IH1'. reflexivity.
-      + destruct (m2 ms' mc) as [r2|] eqn:Heqr2; simpl. 2: constructor.
-        constructor.
-        inversion IH1 as [t1' ms'' gl' res IH1' Heqt1' Heqms'' Heqgl' Heqres | |].
-        clear t1' ms'' gl' res Heqt1' Heqms'' Heqgl' Heqres.
-        simpl. rewrite <- IH1'. simpl.
-        inversion IH2 as [t2' ms''' gl'' res' IH2' Heqt2' Heqms''' Heqgl'' Heqres' | |].
-        clear t2' ms''' gl'' res' Heqt2' Heqms''' Heqgl'' Heqres'. assumption.
-    
-    - (* Quantifier *)
-      intros.
-      remember (Quantified_inner q :: ctx) as ctx'.
-      specialize (IH ctx').
-      destruct Semantics.compileSubPattern as [msub|] eqn:Heqmsub; simpl. 2: discriminate.
-      destruct tCompileSubPattern as [tmsub|] eqn:Heqtmsub; simpl. 2: discriminate.
-      specialize (IH msub tmsub eq_refl eq_refl).
-      simpl in *.
-      destruct negb; simpl. 1: discriminate.
-      unfold equiv_tree_matcher.
-      intros mc tmc gl Hequivcont. unfold equiv_tree_mcont.
-      intro ms.
-      unfold Semantics.repeatMatcher in Heqm.
-      unfold tRepeatMatcher in Heqtm.
-      inversion Heqm as [Heqm'].
-      inversion Heqtm as [Heqtm'].
-      now apply repeatMatcher'_tRepeatMatcher'.
-    
-    - (* Sequence *)
-      intros.
-      remember (Seq_left wr2 :: ctx) as ctxleft.
-      remember (Seq_right wr1 :: ctx) as ctxright.
-      specialize (IH1 ctxleft).
-      specialize (IH2 ctxright).
-      destruct (Semantics.compileSubPattern wr1 _ _ _) as [m1|] eqn:Heqm1; simpl. 2: discriminate.
-      destruct (Semantics.compileSubPattern wr2 _ _ _) as [m2|] eqn:Heqm2; simpl. 2: discriminate.
-      destruct (tCompileSubPattern wr1 _ _ _) as [tm1|] eqn:Heqtm1; simpl. 2: discriminate.
-      destruct (tCompileSubPattern wr2 _ _ _) as [tm2|] eqn:Heqtm2; simpl. 2: discriminate.
-      simpl in *.
-      inversion Heqm as [Heqm'].
-      inversion Heqtm as [Heqtm'].
-      intros mc tmc gl Hequiv ms.
-      specialize (IH2 m2 tm2 eq_refl eq_refl mc tmc gl Hequiv).
-      specialize (IH1 m1 tm1 eq_refl eq_refl (fun ms0 => m2 ms0 mc) (fun ms0 => tm2 ms0 tmc) gl IH2 ms).
-      simpl in *.
-      assumption.
-    
-    - (* Group *)
-      intros.
-      remember (Group_inner name :: ctx) as ctx'.
-      specialize (IH ctx').
-      destruct (Semantics.compileSubPattern wr ctx' rer forward) as [msub|] eqn:Heqmsub; simpl. 2: discriminate.
-      destruct (tCompileSubPattern wr ctx' rer forward) as [tmsub|] eqn:Heqtmsub; simpl. 2: discriminate.
-      intros mc tmc gl Hequiv ms Hmsstr0.
-      simpl in *.
-      inversion Heqm as [Heqm']. clear Heqm Heqm'.
-      inversion Heqtm as [Heqtm']. clear Heqtm Heqtm'.
-      remember (fun y : MatchState => _) as treecont.
-      remember (fun y : MatchState => let! r =<< _ in let! cap =<< _ in mc _) as origcont.
-      remember (StaticSemantics.countLeftCapturingParensBefore _ ctx + 1) as gid.
-      set (gl' := (gid, MatchState.endIndex ms)::gl).
-      specialize (IH msub tmsub eq_refl eq_refl origcont treecont gl').
-      assert (equiv_tree_mcont origcont treecont gl') as Hequivcont.
+Lemma repeatMatcher'_tRepeatMatcher': forall (str0: string) (m: Matcher) (tm: TMatcher),
+  equiv_tree_matcher str0 m tm ->
+  forall fuel: nat,
+  forall (min: non_neg_integer) (max: non_neg_integer_or_inf) (greedy: bool)
+  (parenIndex parenCount: non_neg_integer),
+  equiv_tree_matcher str0
+    (fun ms mc => Semantics.repeatMatcher' m min max greedy ms mc parenIndex parenCount fuel)
+    (fun ms tmc => tRepeatMatcher' tm min max greedy ms tmc parenIndex parenCount fuel).
+Proof.
+  intros str0 m tm Hm_tm_equiv fuel.
+  induction fuel as [|fuel IHfuel].
+  - simpl. constructor.
+  - intros min max greedy parenIndex parenCount mc tmc gl Hequivcont x Hxstr0.
+    simpl.
+    destruct (max =? 0)%NoI eqn:Hmax0; simpl.
+    (* Case max = 0: use hypothesis on continuation *)
+    + unfold equiv_tree_mcont in Hequivcont.
+      now apply Hequivcont.
+    (* Case max > 0 *)
+    + (* Assume that the capture reset succeeds *)
+      destruct List.List.Update.Nat.Batch.update as [cap'|] eqn:Heqcap'; simpl. 2: constructor.
+      remember (match_state (MatchState.input x) (MatchState.endIndex x) cap') as s'.
+      remember (fun y: MatchState => _) as tmc'.
+      remember (fun (y: MatchState) => (_: MatchResult)) as mc'.
+      assert (equiv_tree_mcont str0 mc' tmc' gl) as Hequiv'.
       {
-        intros y Hy_ms_sameinp.
-        rewrite Heqtreecont, Heqorigcont.
-        remember (MatchState.endIndex ms) as i.
-        destruct negb eqn:Hi_le_y; simpl. 1: constructor.
-        destruct (gid =? 0) eqn:Hgid_nonzero; simpl. 1: constructor.
-        destruct List.List.Update.Nat.One.update as [cap'|] eqn:Hcapupd; simpl. 2: constructor.
-        remember (match_state _ _ cap') as ms'.
-        destruct (tmc ms') as [t|] eqn:Heqt; simpl. 2: constructor.
-        destruct (mc ms') as [res|] eqn:Heqres; simpl. 2: constructor.
-        constructor. simpl.
-        rewrite EqDec.reflb. simpl.
-        rewrite Hgid_nonzero.
-        rewrite Hcapupd.
-        specialize (Hequiv ms').
-        assert (MatchState.input ms' = str0) as Hms'str0.
-        {
-          rewrite Heqms'. simpl. apply Hmsstr0.
-        }
-        specialize (Hequiv Hms'str0).
-        rewrite Heqt, Heqres in Hequiv.
-        inversion Hequiv as [t' ms'' gl'' res' Hequiv' Heqt' Heqms'' Heqgl'' Heqres' | |].
-        clear t' ms'' gl'' res' Heqt' Heqms'' Heqgl'' Heqres'.
-        rewrite Heqms' in Hequiv'.
-        rewrite Hy_ms_sameinp.
-        rewrite Hmsstr0 in Hequiv'.
-        assumption.
+        intros s Hsstr0.
+        rewrite Heqmc', Heqtmc'.
+        destruct ((min ==? 0)%wt && _) eqn:Hprogress; simpl.
+        - constructor. reflexivity.
+        - remember (if (min ==? 0)%wt then 0 else min - 1) as min'.
+          remember (if (max =? +∞)%NoI then +∞ else (max - 1)%NoI) as max'.
+          specialize (IHfuel min' max' greedy parenIndex parenCount mc tmc gl Hequivcont s Hsstr0).
+          inversion IHfuel.
+          + simpl. constructor. simpl. assumption.
+          + constructor.
+          + constructor.
       }
-      specialize (IH Hequivcont ms Hmsstr0).
-      simpl in *.
-      destruct (tmsub ms treecont) as [t|] eqn:Heqt; simpl. 2: constructor.
-      destruct (msub ms origcont) as [res|] eqn:Heqres; simpl. 2: constructor.
-      constructor. inversion IH.
-      simpl.
-      assumption.
-    
-    
-    - (* Unsupported *)
-      discriminate.
-    - (* Unsupported *)
-      discriminate.
-    - (* Unsupported *)
-      discriminate.
-    - (* Unsupported *)
-      discriminate.
-    - (* Lookahead: unsupported *)
-      discriminate.
-    - (* Negative lookahead: unsupported *)
-      discriminate.
-    - (* Lookbehind: unsupported *)
-      discriminate.
-    - (* Negative lookbehind: unsupported *)
-      discriminate.
-  Qed.
+      assert (equiv_results (tm s' tmc') s' gl (m s' mc')) as Hequivres.
+      {
+        unfold equiv_tree_matcher in Hm_tm_equiv.
+        specialize (Hm_tm_equiv mc' tmc' gl Hequiv' s').
+        assert (Hs'str0: MatchState.input s' = str0).
+        {
+          rewrite Heqs'. simpl. assumption.
+        }
+        specialize (Hm_tm_equiv Hs'str0).
+        inversion Hm_tm_equiv.
+        2,3: constructor.
+        now constructor.
+      }
+      assert ((reset_groups_ms (seq (parenIndex + 1) parenCount) x) = s') as RESET_GROUPS.
+      {
+        unfold reset_groups_ms.
+        destruct x.
+        rewrite <- List.List.Range.Nat.Length.range_seq.
+        unfold List.List.Range.Nat.Bounds.range in Heqcap'.
+        rewrite decr_range by lia.
+        replace (parenIndex + parenCount + 1 - 1 - (parenIndex + 1 - 1)) with parenCount in Heqcap' by lia.
+        simpl in Heqcap'.
+        rewrite Heqcap'.
+        simpl in *.
+        congruence.
+      }
+      destruct (negb (min =? 0)) eqn:Hmin_nonzero; simpl.
+      (* Case min > 0 *)
+      * inversion Hequivres.
+        2,3: constructor.
+        constructor. simpl.
+        rewrite RESET_GROUPS.
+        simpl.
+        assumption.
+      (* Case min = 0 *)
+      * specialize (Hequivcont x Hxstr0).
+        inversion Hequivcont; inversion Hequivres; destruct greedy eqn:Hgreedy; simpl.
+        all: try constructor.
+        (* There must be a way to make this simpler *)
+        -- subst ms open_gl ms0 open_gl0.
+            rename t0 into z.
+            rename t into z'.
+            rename res0 into zm.
+            unfold "!=?".
+            destruct (zm ==? None)%wt eqn:Hzm_None; simpl.
+            ++ constructor. simpl. rewrite RESET_GROUPS.
+              (* rewrite H8. simpl. *)
+              rewrite EqDec.inversion_true in Hzm_None.
+              rewrite <- H8.
+              rewrite Hzm_None.
+              assumption.
+            ++ constructor. simpl. rewrite RESET_GROUPS.
+              rewrite <- H8. simpl.
+              rewrite EqDec.inversion_false in Hzm_None.
+              destruct zm; simpl.
+              ** reflexivity.
+              ** contradiction.
+        -- subst ms open_gl ms0 open_gl0.
+            rename t0 into z.
+            rename t into z'.
+            rename res0 into zm.
+            rename res into zmc.
+            unfold "!=?".
+            destruct (zmc ==? None)%wt eqn:Hzmc_None; simpl.
+            ++ constructor. simpl. rewrite <- H3. simpl.
+              rewrite EqDec.inversion_true in Hzmc_None.
+              rewrite Hzmc_None.
+              rewrite RESET_GROUPS.
+              simpl.
+              assumption.
+            ++ constructor. simpl. rewrite <- H3. simpl.
+              rewrite EqDec.inversion_false in Hzmc_None.
+              destruct zmc; simpl.
+              ** reflexivity.
+              ** contradiction.
 
-End Main.
+        -- subst ms open_gl ms0 open_gl0.
+            rewrite <- H4.
+            destruct t'.
+            ++ simpl.
+              unfold "!=?".
+              destruct (res ==? None)%wt eqn:Hres_None; simpl.
+              ** constructor.
+              ** constructor. simpl. rewrite <- H3.
+                  simpl.
+                  rewrite EqDec.inversion_false in Hres_None.
+                  destruct res.
+                  --- reflexivity.
+                  --- contradiction.
+            ++ simpl. constructor.
+
+        -- subst ms open_gl ms0 open_gl0.
+            rewrite <- H.
+            destruct t'.
+            ++ simpl.
+              unfold "!=?".
+              destruct (res ==? None)%wt eqn:Hres_None; simpl.
+              ** constructor.
+              ** constructor. simpl. rewrite RESET_GROUPS.
+                  rewrite <- H7. simpl.
+                  rewrite EqDec.inversion_false in Hres_None.
+                  now destruct res.
+            ++ simpl. constructor.
+Qed.
+
+
+Theorem compile_tcompile: forall reg ctx rer m tm
+  (Heqm: Semantics.compileSubPattern reg ctx rer forward = Success m)
+  (Heqtm: tCompileSubPattern reg ctx rer forward = Success tm),
+  forall str0, equiv_tree_matcher str0 m tm.
+Proof.
+  intros reg ctx rer.
+  revert ctx.
+  induction reg as [
+    |
+    chr |
+    |
+    ae |
+    cc |
+    wr1 IH1 wr2 IH2 |
+    wr IH q |
+    wr1 IH1 wr2 IH2 |
+    name wr IH |
+    |
+    |
+    |
+    |
+    wr IH |
+    wr IH |
+    wr IH |
+    wr IH
+  ]; simpl.
+
+  - (* Empty *)
+    intros. inversion Heqm as [Heqm']. inversion Heqtm as [Heqtm'].
+    intros mc tmc gl Hequiv ms Hmsstr0.
+    apply Hequiv. assumption.
+
+  - (* Character *)
+    intros. unfold equiv_tree_matcher. intros mc tmc gl Hequiv ms Hmsstr0.
+    inversion Heqtm as [Heqtm']. clear Heqtm Heqtm'.
+    inversion Heqm as [Heqm']. clear Heqm Heqm'.
+    unfold tCharacterSetMatcher, Semantics.characterSetMatcher.
+    simpl.
+    remember ((_ <? 0)%Z || _) as oob.
+    destruct oob eqn:Hoob.
+    + constructor. reflexivity.
+    + remember (Z.min _ _) as index.
+      remember (List.List.Indexing.Int.indexing _ _) as readchr.
+      destruct readchr as [readchr|]; simpl. 2: constructor.
+      remember (CharSet.exist_canonicalized _ _ _) as read_matches.
+      destruct read_matches eqn:Hread_matches; simpl.
+      2: constructor; reflexivity.
+      remember (match_state _ _ _) as ms'.
+      specialize (Hequiv ms').
+      assert (MatchState.input ms' = str0) as Hms'str0.
+      {
+        rewrite Heqms'. simpl. apply Hmsstr0.
+      }
+      specialize (Hequiv Hms'str0).
+      destruct (tmc ms') as [child|]; simpl. 2: constructor.
+      destruct (mc ms') as [res|]; simpl. 2: constructor.
+      constructor.
+      replace (Z.min (MatchState.endIndex ms) (MatchState.endIndex ms + 1)) with (MatchState.endIndex ms) in Heqindex by lia.
+      rewrite Heqindex in Heqreadchr.
+      simpl.
+      inversion Hequiv as [child0 ms'0 gl0 res0 Hequiv' Heqchild0 Heqms'0 Heqgl0 Heqres0 | |].
+      unfold advance_ms.
+      rewrite <- Heqms'.
+      rewrite <- Hequiv'.
+      reflexivity.
+
+  - (* Dot; same as character *)
+    intros. unfold equiv_tree_matcher. intros mc tmc gl Hequiv ms Hmsstr0.
+    inversion Heqtm as [Heqtm']. clear Heqtm Heqtm'.
+    inversion Heqm as [Heqm']. clear Heqm Heqm'.
+    unfold tCharacterSetMatcher, Semantics.characterSetMatcher.
+    simpl.
+    remember ((_ <? 0)%Z || _) as oob.
+    destruct oob eqn:Hoob.
+    + constructor. reflexivity.
+    + remember (Z.min _ _) as index.
+      remember (List.List.Indexing.Int.indexing _ _) as readchr.
+      destruct readchr as [readchr|]; simpl. 2: constructor.
+      remember (CharSet.exist_canonicalized _ _ _) as read_matches.
+      destruct read_matches eqn:Hread_matches; simpl.
+      2: constructor; reflexivity.
+      remember (match_state _ _ _) as ms'.
+      specialize (Hequiv ms').
+      assert (MatchState.input ms' = str0) as Hms'str0.
+      {
+        rewrite Heqms'. simpl. apply Hmsstr0.
+      }
+      specialize (Hequiv Hms'str0).
+      destruct (tmc ms') as [child|]; simpl. 2: constructor.
+      destruct (mc ms') as [res|]; simpl. 2: constructor.
+      constructor.
+      replace (Z.min (MatchState.endIndex ms) (MatchState.endIndex ms + 1)) with (MatchState.endIndex ms) in Heqindex by lia.
+      rewrite Heqindex in Heqreadchr.
+      simpl.
+      inversion Hequiv as [child0 ms'0 gl0 res0 Hequiv' Heqchild0 Heqms'0 Heqgl0 Heqres0 | |].
+      unfold advance_ms.
+      rewrite <- Heqms'.
+      rewrite <- Hequiv'.
+      reflexivity.
+
+  - (* Atom escape: unsupported *)
+    intros. destruct (match ae with | DecimalEsc de => _ | ACharacterClassEsc cce => _ | ACharacterEsc ce => _ | GroupEsc gn => _ end); discriminate.
+
+  - (* Character class: unsupported *)
+    intros. destruct (let! _ =<< _ in _); discriminate.
+
+  - (* Disjunction *)
+    intros.
+    remember (Disjunction_left wr2 :: ctx) as ctxleft.
+    remember (Disjunction_right wr1 :: ctx) as ctxright.
+    specialize (IH1 ctxleft).
+    specialize (IH2 ctxright).
+    destruct (Semantics.compileSubPattern wr1 _ _ _) as [m1|] eqn:Heqm1; simpl. 2: discriminate.
+    destruct (Semantics.compileSubPattern wr2 _ _ _) as [m2|] eqn:Heqm2; simpl. 2: discriminate.
+    destruct (tCompileSubPattern wr1 _ _ _) as [tm1|] eqn:Heqtm1; simpl. 2: discriminate.
+    destruct (tCompileSubPattern wr2 _ _ _) as [tm2|] eqn:Heqtm2; simpl. 2: discriminate.
+    simpl in *.
+    unfold equiv_tree_matcher.
+    intros mc tmc gl Hequiv ms' Hms'str0.
+    specialize (IH1 m1 tm1 eq_refl eq_refl str0 mc tmc gl Hequiv ms' Hms'str0).
+    specialize (IH2 m2 tm2 eq_refl eq_refl str0 mc tmc gl Hequiv ms' Hms'str0).
+    simpl in *.
+    inversion Heqtm as [Heqtm'].
+    destruct (tm1 ms' tmc) as [t1|] eqn:Heqt1; simpl. 2: constructor.
+    destruct (tm2 ms' tmc) as [t2|] eqn:Heqt2; simpl. 2: constructor.
+    inversion Heqm as [Heqm'].
+    destruct (m1 ms' mc) as [r|] eqn:Heqr; simpl. 2: constructor.
+    destruct r eqn:?; simpl.
+    + constructor. inversion IH1 as [t1' ms'' gl' res IH1' Heqt1' Heqms'' Heqgl' Heqres | |].
+      simpl. rewrite <- IH1'. reflexivity.
+    + destruct (m2 ms' mc) as [r2|] eqn:Heqr2; simpl. 2: constructor.
+      constructor.
+      inversion IH1 as [t1' ms'' gl' res IH1' Heqt1' Heqms'' Heqgl' Heqres | |].
+      clear t1' ms'' gl' res Heqt1' Heqms'' Heqgl' Heqres.
+      simpl. rewrite <- IH1'. simpl.
+      inversion IH2 as [t2' ms''' gl'' res' IH2' Heqt2' Heqms''' Heqgl'' Heqres' | |].
+      clear t2' ms''' gl'' res' Heqt2' Heqms''' Heqgl'' Heqres'. assumption.
+
+  - (* Quantifier *)
+    intros.
+    remember (Quantified_inner q :: ctx) as ctx'.
+    specialize (IH ctx').
+    destruct Semantics.compileSubPattern as [msub|] eqn:Heqmsub; simpl. 2: discriminate.
+    destruct tCompileSubPattern as [tmsub|] eqn:Heqtmsub; simpl. 2: discriminate.
+    specialize (IH msub tmsub eq_refl eq_refl).
+    simpl in *.
+    destruct negb; simpl. 1: discriminate.
+    unfold equiv_tree_matcher.
+    intros mc tmc gl Hequivcont. unfold equiv_tree_mcont.
+    intro ms.
+    unfold Semantics.repeatMatcher in Heqm.
+    unfold tRepeatMatcher in Heqtm.
+    inversion Heqm as [Heqm'].
+    inversion Heqtm as [Heqtm'].
+    now apply repeatMatcher'_tRepeatMatcher'.
+
+  - (* Sequence *)
+    intros.
+    remember (Seq_left wr2 :: ctx) as ctxleft.
+    remember (Seq_right wr1 :: ctx) as ctxright.
+    specialize (IH1 ctxleft).
+    specialize (IH2 ctxright).
+    destruct (Semantics.compileSubPattern wr1 _ _ _) as [m1|] eqn:Heqm1; simpl. 2: discriminate.
+    destruct (Semantics.compileSubPattern wr2 _ _ _) as [m2|] eqn:Heqm2; simpl. 2: discriminate.
+    destruct (tCompileSubPattern wr1 _ _ _) as [tm1|] eqn:Heqtm1; simpl. 2: discriminate.
+    destruct (tCompileSubPattern wr2 _ _ _) as [tm2|] eqn:Heqtm2; simpl. 2: discriminate.
+    simpl in *.
+    inversion Heqm as [Heqm'].
+    inversion Heqtm as [Heqtm'].
+    intros mc tmc gl Hequiv ms.
+    specialize (IH2 m2 tm2 eq_refl eq_refl str0 mc tmc gl Hequiv).
+    specialize (IH1 m1 tm1 eq_refl eq_refl str0 (fun ms0 => m2 ms0 mc) (fun ms0 => tm2 ms0 tmc) gl IH2 ms).
+    simpl in *.
+    assumption.
+
+  - (* Group *)
+    intros.
+    remember (Group_inner name :: ctx) as ctx'.
+    specialize (IH ctx').
+    destruct (Semantics.compileSubPattern wr ctx' rer forward) as [msub|] eqn:Heqmsub; simpl. 2: discriminate.
+    destruct (tCompileSubPattern wr ctx' rer forward) as [tmsub|] eqn:Heqtmsub; simpl. 2: discriminate.
+    intros mc tmc gl Hequiv ms Hmsstr0.
+    simpl in *.
+    inversion Heqm as [Heqm']. clear Heqm Heqm'.
+    inversion Heqtm as [Heqtm']. clear Heqtm Heqtm'.
+    remember (fun y : MatchState => _) as treecont.
+    remember (fun y : MatchState => let! r =<< _ in let! cap =<< _ in mc _) as origcont.
+    remember (StaticSemantics.countLeftCapturingParensBefore _ ctx + 1) as gid.
+    set (gl' := (gid, MatchState.endIndex ms)::gl).
+    specialize (IH msub tmsub eq_refl eq_refl str0 origcont treecont gl').
+    assert (equiv_tree_mcont str0 origcont treecont gl') as Hequivcont.
+    {
+      intros y Hy_ms_sameinp.
+      rewrite Heqtreecont, Heqorigcont.
+      remember (MatchState.endIndex ms) as i.
+      destruct negb eqn:Hi_le_y; simpl. 1: constructor.
+      destruct (gid =? 0) eqn:Hgid_nonzero; simpl. 1: constructor.
+      destruct List.List.Update.Nat.One.update as [cap'|] eqn:Hcapupd; simpl. 2: constructor.
+      remember (match_state _ _ cap') as ms'.
+      destruct (tmc ms') as [t|] eqn:Heqt; simpl. 2: constructor.
+      destruct (mc ms') as [res|] eqn:Heqres; simpl. 2: constructor.
+      constructor. simpl.
+      rewrite EqDec.reflb. simpl.
+      rewrite Hgid_nonzero.
+      rewrite Hcapupd.
+      specialize (Hequiv ms').
+      assert (MatchState.input ms' = str0) as Hms'str0.
+      {
+        rewrite Heqms'. simpl. apply Hmsstr0.
+      }
+      specialize (Hequiv Hms'str0).
+      rewrite Heqt, Heqres in Hequiv.
+      inversion Hequiv as [t' ms'' gl'' res' Hequiv' Heqt' Heqms'' Heqgl'' Heqres' | |].
+      clear t' ms'' gl'' res' Heqt' Heqms'' Heqgl'' Heqres'.
+      rewrite Heqms' in Hequiv'.
+      rewrite Hy_ms_sameinp.
+      rewrite Hmsstr0 in Hequiv'.
+      assumption.
+    }
+    specialize (IH Hequivcont ms Hmsstr0).
+    simpl in *.
+    destruct (tmsub ms treecont) as [t|] eqn:Heqt; simpl. 2: constructor.
+    destruct (msub ms origcont) as [res|] eqn:Heqres; simpl. 2: constructor.
+    constructor. inversion IH.
+    simpl.
+    assumption.
+
+
+  - (* Unsupported *)
+    discriminate.
+  - (* Unsupported *)
+    discriminate.
+  - (* Unsupported *)
+    discriminate.
+  - (* Unsupported *)
+    discriminate.
+  - (* Lookahead: unsupported *)
+    discriminate.
+  - (* Negative lookahead: unsupported *)
+    discriminate.
+  - (* Lookbehind: unsupported *)
+    discriminate.
+  - (* Negative lookbehind: unsupported *)
+    discriminate.
+Qed.
