warblreequiv/LWEquivTree.v
@@ -86,7 +86,7 @@ Definition tMC_is_tree (tmc: TMatcherContinuation) (rer: RegExpRecord) (lreg: re
 Definition tMC_valid (tmc: TMatcherContinuation) (rer: RegExpRecord) (lreg: regex) (cont: continuation) (str0: string) :=
   forall inp, input_compat inp str0 -> tMC_is_tree tmc rer lreg cont inp.
 
-(* `tm_valid tm rer lreg` means that the TMatcher tm recognizes the regexp lreg on any input, and yields a valid backtree. *)
+(* `tm_valid tm rer lreg` means that under the given RegExpRecord (set of flags), the TMatcher tm recognizes the regexp lreg on any input, and yields a valid backtree. *)
 Definition tm_valid (tm: TMatcher) (rer: RegExpRecord) (lreg: regex) :=
   forall (tmc: TMatcherContinuation) (lregc: regex) (cont: continuation) (str0: string),
   tMC_valid tmc rer lregc cont str0 ->
@@ -197,278 +197,274 @@ Admitted.
 
 
 
-Section Main.
-  Context (str0: string) (rer: RegExpRecord) (lroot: regex) (wroot: Regex).
-  Hypothesis Hcasesenst: RegExpRecord.ignoreCase rer = false.
-  Hypothesis root_equiv: equiv_regex wroot lroot.
-
-
-  (* Theorem is not true for case-insensitive matching, which is not supported (yet) by the tree semantics *)
-  (* Validity of the context and regexp? *)
-  Theorem tmatcher_bt: forall wreg lreg ctx,
+(* Theorem is not true for case-insensitive matching, which is not supported (yet) by the tree semantics *)
+(* Validity of the context and regexp? *)
+Theorem tmatcher_bt:
+  forall (str0: string) (rer: RegExpRecord) (lroot: regex) (wroot: Regex)
+    (Hcasesenst: RegExpRecord.ignoreCase rer = false)
+    (root_equiv: equiv_regex wroot lroot),
+  forall (wreg: Regex) (lreg: regex) ctx,
     equiv_regex wreg lreg ->
     Root wroot (wreg, ctx) ->
-    forall tm,
-      tCompileSubPattern wreg ctx rer forward = Success tm ->
-      tm_valid tm lreg.
-  Proof.
-    intros wreg lreg ctx Hequiv.
-    revert ctx.
-    induction Hequiv as [
-      n |
-      n c |
-      n |
-      n wr1 wr2 lr1 lr2 Hequiv1 IH1 Hequiv2 IH2 |
-      n wr1 wr2 lr1 lr2 Hequiv1 IH1 Hequiv2 IH2 |
-      n wr lr Hequiv IH |
-      n wr lr Hequiv IH |
-      name n wr lr Hequiv IH
-    ].
+  forall tm,
+    tCompileSubPattern wreg ctx rer forward = Success tm ->
+    tm_valid tm rer lreg.
+Proof.
+  intros wreg lreg ctx Hequiv.
+  revert ctx.
+  induction Hequiv as [
+    n |
+    n c |
+    n |
+    n wr1 wr2 lr1 lr2 Hequiv1 IH1 Hequiv2 IH2 |
+    n wr1 wr2 lr1 lr2 Hequiv1 IH1 Hequiv2 IH2 |
+    n wr lr Hequiv IH |
+    n wr lr Hequiv IH |
+    name n wr lr Hequiv IH
+  ].
 
 
-    - (* Empty *)
-      simpl. intros _ _.
-      intros tmc regc cont Htmc_tree inp Hinp_compat.
-      unfold tMC_is_tree.
-      intros s Hvalids Hs_inp.
-      specialize (Htmc_tree inp Hinp_compat s Hvalids Hs_inp).
-      destruct (tmc s) as [t|] eqn:Heqtmc; simpl; try exact I.
-      apply tree_pop_reg. assumption.
-    
+  - (* Empty *)
+    simpl. intros _ _.
+    intros tmc regc cont Htmc_tree inp Hinp_compat.
+    unfold tMC_is_tree.
+    intros s Hvalids Hs_inp.
+    specialize (Htmc_tree inp Hinp_compat s Hvalids Hs_inp).
+    destruct (tmc s) as [t|] eqn:Heqtmc; simpl; try exact I.
+    apply tree_pop_reg. assumption.
 
-    - (* Character *)
-      simpl.
-      intro ctx.
-      intros Hroot tmc regc cont Htmc_tree inp Hinp_compat.
-      (*specialize (Htmc_tree inp Hinp_compat).*)
-      unfold tMC_is_tree.
-      intros s Hsvalid Hs_inp.
-      destruct tCharacterSetMatcher as [t|e] eqn:Heqmatcher; simpl. 2: exact I.
-      unfold tCharacterSetMatcher in Heqmatcher.
-      simpl in Heqmatcher.
-      set (next_outofbounds := (_ <? 0)%Z || _) in Heqmatcher.
-      destruct next_outofbounds eqn:Hoob; simpl.
-      * inversion Heqmatcher.
-        apply tree_char_fail.
-        (* Reading out of bounds fails *)
-        admit.
-      * replace (Z.min _ _) with (@MatchState.endIndex Chars.Char char_marker s) in Heqmatcher by lia.
-        destruct List.List.Indexing.Int.indexing as [chr|err] eqn:Hgetchr; simpl.
-        -- simpl in Heqmatcher.
-           destruct CharSet.exist_canonicalized eqn:Hcharmatch; simpl.
-           ++ remember (match_state _ _ _) as s' in Heqmatcher.
-              unfold tMC_is_tree in Htmc_tree.
-              assert (Valid (MatchState.input s') rer s') as Hs'valid by admit.
-              set (inp'_opt := advance_input inp).
-              destruct inp'_opt as [inp'|] eqn:Heqinp'.
-              2: { exfalso; admit. }
-              assert (ms_matches_inp s' inp') as Hs'_inp' by admit.
-              assert (input_compat inp') as Hinp'_compat by admit.
-              specialize (Htmc_tree inp' Hinp'_compat s' Hs'valid Hs'_inp').
-              destruct (tmc s') as [child|] eqn:Heqtmc; simpl; try discriminate.
-              simpl in Heqmatcher.
-              inversion Heqmatcher.
-              admit.
-           ++ admit.
-        -- discriminate.
-    
-      (* Dot *)
-    - simpl.
+
+  - (* Character *)
+    simpl.
+    intro ctx.
+    intros Hroot tmc regc cont Htmc_tree inp Hinp_compat.
+    (*specialize (Htmc_tree inp Hinp_compat).*)
+    unfold tMC_is_tree.
+    intros s Hsvalid Hs_inp.
+    destruct tCharacterSetMatcher as [t|e] eqn:Heqmatcher; simpl. 2: exact I.
+    unfold tCharacterSetMatcher in Heqmatcher.
+    simpl in Heqmatcher.
+    set (next_outofbounds := (_ <? 0)%Z || _) in Heqmatcher.
+    destruct next_outofbounds eqn:Hoob; simpl.
+    * inversion Heqmatcher.
+      apply tree_char_fail.
+      (* Reading out of bounds fails *)
       admit.
-      
+    * replace (Z.min _ _) with (@MatchState.endIndex Chars.Char char_marker s) in Heqmatcher by lia.
+      destruct List.List.Indexing.Int.indexing as [chr|err] eqn:Hgetchr; simpl.
+      -- simpl in Heqmatcher.
+         destruct CharSet.exist_canonicalized eqn:Hcharmatch; simpl.
+         ++ remember (match_state _ _ _) as s' in Heqmatcher.
+            unfold tMC_is_tree in Htmc_tree.
+            assert (Valid (MatchState.input s') rer s') as Hs'valid by admit.
+            set (inp'_opt := advance_input inp).
+            destruct inp'_opt as [inp'|] eqn:Heqinp'.
+            2: { exfalso; admit. }
+            assert (ms_matches_inp s' inp') as Hs'_inp' by admit.
+            assert (input_compat inp') as Hinp'_compat by admit.
+            specialize (Htmc_tree inp' Hinp'_compat s' Hs'valid Hs'_inp').
+            destruct (tmc s') as [child|] eqn:Heqtmc; simpl; try discriminate.
+            simpl in Heqmatcher.
+            inversion Heqmatcher.
+            admit.
+         ++ admit.
+      -- discriminate.
 
-    - (* Disjunction *)
-      intro ctx.
-      simpl in *.
-      intro Hroot.
-      remember (@Disjunction_left LindenParameters wr2 :: ctx) as ctx1.
-      remember (@Disjunction_right LindenParameters wr1 :: ctx) as ctx2.
-      specialize (IH1 ctx1).
-      specialize (IH2 ctx2).
-      assert (Root wroot (wr1, ctx1)) as Hroot1.
-      {
-        rewrite Heqctx1.
-        apply same_root_down0 with (r1 := Disjunction wr1 wr2) (ctx1 := ctx).
-        - apply (@Down_Disjunction_left LindenParameters).
-        - apply Hroot.
-      }
-      assert (Root wroot (wr2, ctx2)) as Hroot2.
-      {
-        apply same_root_down0 with (r1 := Disjunction wr1 wr2) (ctx1 := ctx).
-        - rewrite Heqctx2. apply (@Down_Disjunction_right LindenParameters).
-        - apply Hroot.
-      }
-      specialize (IH1 Hroot1).
-      specialize (IH2 Hroot2).
-      destruct (tCompileSubPattern wr1 ctx1 rer forward) as [tm1|] eqn:Htm1; simpl; try exact I.
-      destruct (tCompileSubPattern wr2 ctx2 rer forward) as [tm2|] eqn:Htm2; simpl; try exact I.
-      intros tmc regc cont Htmc_tree inp Hinp_compat.
+    (* Dot *)
+  - simpl.
+    admit.
+
+
+  - (* Disjunction *)
+    intro ctx.
+    simpl in *.
+    intro Hroot.
+    remember (@Disjunction_left LindenParameters wr2 :: ctx) as ctx1.
+    remember (@Disjunction_right LindenParameters wr1 :: ctx) as ctx2.
+    specialize (IH1 ctx1).
+    specialize (IH2 ctx2).
+    assert (Root wroot (wr1, ctx1)) as Hroot1.
+    {
+      rewrite Heqctx1.
+      apply same_root_down0 with (r1 := Disjunction wr1 wr2) (ctx1 := ctx).
+      - apply (@Down_Disjunction_left LindenParameters).
+      - apply Hroot.
+    }
+    assert (Root wroot (wr2, ctx2)) as Hroot2.
+    {
+      apply same_root_down0 with (r1 := Disjunction wr1 wr2) (ctx1 := ctx).
+      - rewrite Heqctx2. apply (@Down_Disjunction_right LindenParameters).
+      - apply Hroot.
+    }
+    specialize (IH1 Hroot1).
+    specialize (IH2 Hroot2).
+    destruct (tCompileSubPattern wr1 ctx1 rer forward) as [tm1|] eqn:Htm1; simpl; try exact I.
+    destruct (tCompileSubPattern wr2 ctx2 rer forward) as [tm2|] eqn:Htm2; simpl; try exact I.
+    intros tmc regc cont Htmc_tree inp Hinp_compat.
+    unfold tMC_is_tree.
+    intros s Hsvalid Hs_inp.
+    specialize (IH1 tmc regc cont Htmc_tree inp Hinp_compat).
+    specialize (IH2 tmc regc cont Htmc_tree inp Hinp_compat).
+    unfold tMC_is_tree in IH1, IH2.
+    specialize (IH1 s Hsvalid Hs_inp).
+    specialize (IH2 s Hsvalid Hs_inp).
+    destruct (tm1 s tmc) as [t1|] eqn:Heqt1; simpl; try exact I.
+    destruct (tm2 s tmc) as [t2|] eqn:Heqt2; simpl; try exact I.
+    now apply tree_disj.
+    (* DONE! 🎉 *)
+
+
+  - (* Sequence *)
+    intro ctx.
+    simpl in *.
+    intro Hroot.
+    remember (@Seq_left LindenParameters wr2 :: ctx) as ctx1.
+    remember (@Seq_right LindenParameters wr1 :: ctx) as ctx2.
+    specialize (IH1 ctx1).
+    specialize (IH2 ctx2).
+    assert (Root wroot (wr1, ctx1)) as Hroot1.
+    {
+      apply same_root_down0 with (r1 := Seq wr1 wr2) (ctx1 := ctx).
+      - rewrite Heqctx1. apply (@Down_Seq_left LindenParameters).
+      - apply Hroot.
+    }
+    assert (Root wroot (wr2, ctx2)) as Hroot2.
+    {
+      apply same_root_down0 with (r1 := Seq wr1 wr2) (ctx1 := ctx).
+      - rewrite Heqctx2. apply (@Down_Seq_right LindenParameters).
+      - apply Hroot.
+    }
+    specialize (IH1 Hroot1).
+    specialize (IH2 Hroot2).
+    destruct (tCompileSubPattern wr1 ctx1 rer forward) as [tm1|] eqn:Htm1; simpl; try exact I.
+    destruct (tCompileSubPattern wr2 ctx2 rer forward) as [tm2|] eqn:Htm2; simpl; try exact I.
+    intros tmc regc cont Htmc_tree inp Hinp_compat.
+    unfold tMC_is_tree.
+    intros s Hsvalid Hs_inp.
+    remember (fun s1 => tm2 s1 tmc) as tmc2.
+    assert (forall inp': input, input_compat inp' -> tMC_is_tree tmc2 lr2 (Areg regc :: cont) inp') as Htmc2_tree.
+    {
+      intros inp' Hinp'_compat.
+      rewrite Heqtmc2.
+      now apply IH2.
+    }
+    specialize (IH1 tmc2 lr2 (Areg regc :: cont) Htmc2_tree inp Hinp_compat).
+    unfold tMC_is_tree in IH1.
+    specialize (IH1 s Hsvalid Hs_inp).
+    destruct (tm1 s tmc2) as [t|] eqn:Heqt; simpl; try exact I.
+    now apply tree_sequence.
+    (* DONE! 🎉 *)
+
+
+  - (* Lazy star *)
+    intros ctx Hroot.
+    simpl.
+    destruct tCompileSubPattern as [m|] eqn:Heqm; simpl. 2: exact I.
+    intros tmc regc cont Htmc_valid.
+    pose proof tRepeatMatcher'_valid false (StaticSemantics.countLeftCapturingParensBefore wr ctx)
+    (StaticSemantics.countLeftCapturingParensWithin wr (Quantified_inner (Lazy Star) :: ctx)) m lr as Hrepeat.
+    specialize (IH (Quantified_inner (Lazy Star)::ctx)).
+    assert (Root wroot (wr, Quantified_inner (Lazy Star)::ctx)) as Hroot1 by
+      eauto using same_root_down0, Down_Quantified_inner.
+    specialize (IH Hroot1).
+    rewrite Heqm in IH.
+    specialize (Hrepeat IH).
+    remember (StaticSemantics.countLeftCapturingParensBefore _ ctx) as parenIndex.
+    remember (StaticSemantics.countLeftCapturingParensWithin _ _) as parenCount.
+    assert (def_groups lr = seq (parenIndex + 1) parenCount) as Hgroups_valid by admit.
+    specialize (Hrepeat Hgroups_valid).
+    unfold tMC_valid.
+    intros inp Hinp_compat.
+    unfold tMC_is_tree.
+    intros s Hvalids Hs_inp.
+    specialize (Hrepeat (Semantics.repeatMatcherFuel 0 s)).
+    unfold tm_valid in Hrepeat.
+    specialize (Hrepeat tmc regc cont Htmc_valid).
+    now apply Hrepeat.
+
+    (* Greedy star: copy-pasting... *)
+  - intros ctx Hroot.
+    simpl.
+    destruct tCompileSubPattern as [m|] eqn:Heqm; simpl. 2: exact I.
+    intros tmc regc cont Htmc_valid.
+    pose proof tRepeatMatcher'_valid true (StaticSemantics.countLeftCapturingParensBefore wr ctx)
+    (StaticSemantics.countLeftCapturingParensWithin wr (Quantified_inner (Greedy Star) :: ctx)) m lr as Hrepeat.
+    specialize (IH (Quantified_inner (Greedy Star)::ctx)).
+    assert (Root wroot (wr, Quantified_inner (Greedy Star)::ctx)) as Hroot1.
+    {
+      eapply same_root_down0.
+      - apply (@Down_Quantified_inner LindenParameters).
+      - apply Hroot.
+    }
+    specialize (IH Hroot1).
+    rewrite Heqm in IH.
+    specialize (Hrepeat IH).
+    remember (StaticSemantics.countLeftCapturingParensBefore _ ctx) as parenIndex.
+    remember (StaticSemantics.countLeftCapturingParensWithin _ _) as parenCount.
+    assert (def_groups lr = seq (parenIndex + 1) parenCount) as Hgroups_valid by admit.
+    specialize (Hrepeat Hgroups_valid).
+    unfold tMC_valid.
+    intros inp Hinp_compat.
+    unfold tMC_is_tree.
+    intros s Hvalids Hs_inp.
+    specialize (Hrepeat (Semantics.repeatMatcherFuel 0 s)).
+    unfold tm_valid in Hrepeat.
+    specialize (Hrepeat tmc regc cont Htmc_valid).
+    now apply Hrepeat.
+
+
+  - (* Group *)
+    intros ctx Hroot. simpl.
+    remember (@Group_inner LindenParameters _ :: ctx) as rctx.
+    specialize (IH rctx).
+    assert (Root wroot (wr, rctx)) as Hrootr.
+    {
+      eapply same_root_down0.
+      - subst rctx. apply (@Down_Group_inner LindenParameters).
+      - apply Hroot.
+    }
+    specialize (IH Hrootr).
+    destruct (tCompileSubPattern wr rctx rer forward) as [mr|] eqn:Heqmr; simpl; try exact I.
+    intros tmc regc cont Htmc_tree inp Hinp_compat.
+    unfold tMC_is_tree.
+    intros s Hvalids Hs_inp.
+    remember (fun y: MatchState => _) as tmc2.
+    (* Let's try something *)
+    specialize (IH tmc2 Epsilon (Aclose (S n) :: Areg regc :: cont)).
+    assert (StaticSemantics.countLeftCapturingParensBefore (Group name wr) ctx + 1 = S n) as Heqid by admit.
+    assert (forall inp : input, input_compat inp -> tMC_is_tree tmc2 Epsilon (Aclose (S n) :: Areg regc :: cont) inp) as Htmc2_tree.
+    {
+      intros inp' Hinp'_compat.
+      rewrite Heqtmc2.
       unfold tMC_is_tree.
-      intros s Hsvalid Hs_inp.
-      specialize (IH1 tmc regc cont Htmc_tree inp Hinp_compat).
-      specialize (IH2 tmc regc cont Htmc_tree inp Hinp_compat).
-      unfold tMC_is_tree in IH1, IH2.
-      specialize (IH1 s Hsvalid Hs_inp).
-      specialize (IH2 s Hsvalid Hs_inp).
-      destruct (tm1 s tmc) as [t1|] eqn:Heqt1; simpl; try exact I.
-      destruct (tm2 s tmc) as [t2|] eqn:Heqt2; simpl; try exact I.
-      now apply tree_disj.
-      (* DONE! 🎉 *)
-
-
-    - (* Sequence *)
-      intro ctx.
-      simpl in *.
-      intro Hroot.
-      remember (@Seq_left LindenParameters wr2 :: ctx) as ctx1.
-      remember (@Seq_right LindenParameters wr1 :: ctx) as ctx2.
-      specialize (IH1 ctx1).
-      specialize (IH2 ctx2).
-      assert (Root wroot (wr1, ctx1)) as Hroot1.
-      {
-        apply same_root_down0 with (r1 := Seq wr1 wr2) (ctx1 := ctx).
-        - rewrite Heqctx1. apply (@Down_Seq_left LindenParameters).
-        - apply Hroot.
-      }
-      assert (Root wroot (wr2, ctx2)) as Hroot2.
-      {
-        apply same_root_down0 with (r1 := Seq wr1 wr2) (ctx1 := ctx).
-        - rewrite Heqctx2. apply (@Down_Seq_right LindenParameters).
-        - apply Hroot.
-      }
-      specialize (IH1 Hroot1).
-      specialize (IH2 Hroot2).
-      destruct (tCompileSubPattern wr1 ctx1 rer forward) as [tm1|] eqn:Htm1; simpl; try exact I.
-      destruct (tCompileSubPattern wr2 ctx2 rer forward) as [tm2|] eqn:Htm2; simpl; try exact I.
-      intros tmc regc cont Htmc_tree inp Hinp_compat.
-      unfold tMC_is_tree.
-      intros s Hsvalid Hs_inp.
-      remember (fun s1 => tm2 s1 tmc) as tmc2.
-      assert (forall inp': input, input_compat inp' -> tMC_is_tree tmc2 lr2 (Areg regc :: cont) inp') as Htmc2_tree.
-      {
-        intros inp' Hinp'_compat.
-        rewrite Heqtmc2.
-        now apply IH2.
-      }
-      specialize (IH1 tmc2 lr2 (Areg regc :: cont) Htmc2_tree inp Hinp_compat).
-      unfold tMC_is_tree in IH1.
-      specialize (IH1 s Hsvalid Hs_inp).
-      destruct (tm1 s tmc2) as [t|] eqn:Heqt; simpl; try exact I.
-      now apply tree_sequence.
-      (* DONE! 🎉 *)
-
-
-    - (* Lazy star *)
-      intros ctx Hroot.
-      simpl.
-      destruct tCompileSubPattern as [m|] eqn:Heqm; simpl. 2: exact I.
-      intros tmc regc cont Htmc_valid.
-      pose proof tRepeatMatcher'_valid false (StaticSemantics.countLeftCapturingParensBefore wr ctx)
-      (StaticSemantics.countLeftCapturingParensWithin wr (Quantified_inner (Lazy Star) :: ctx)) m lr as Hrepeat.
-      specialize (IH (Quantified_inner (Lazy Star)::ctx)).
-      assert (Root wroot (wr, Quantified_inner (Lazy Star)::ctx)) as Hroot1 by
-        eauto using same_root_down0, Down_Quantified_inner.
-      specialize (IH Hroot1).
-      rewrite Heqm in IH.
-      specialize (Hrepeat IH).
-      remember (StaticSemantics.countLeftCapturingParensBefore _ ctx) as parenIndex.
-      remember (StaticSemantics.countLeftCapturingParensWithin _ _) as parenCount.
-      assert (def_groups lr = seq (parenIndex + 1) parenCount) as Hgroups_valid by admit.
-      specialize (Hrepeat Hgroups_valid).
-      unfold tMC_valid.
-      intros inp Hinp_compat.
-      unfold tMC_is_tree.
-      intros s Hvalids Hs_inp.
-      specialize (Hrepeat (Semantics.repeatMatcherFuel 0 s)).
-      unfold tm_valid in Hrepeat.
-      specialize (Hrepeat tmc regc cont Htmc_valid).
-      now apply Hrepeat.
-      
-      (* Greedy star: copy-pasting... *)
-    - intros ctx Hroot.
-      simpl.
-      destruct tCompileSubPattern as [m|] eqn:Heqm; simpl. 2: exact I.
-      intros tmc regc cont Htmc_valid.
-      pose proof tRepeatMatcher'_valid true (StaticSemantics.countLeftCapturingParensBefore wr ctx)
-      (StaticSemantics.countLeftCapturingParensWithin wr (Quantified_inner (Greedy Star) :: ctx)) m lr as Hrepeat.
-      specialize (IH (Quantified_inner (Greedy Star)::ctx)).
-      assert (Root wroot (wr, Quantified_inner (Greedy Star)::ctx)) as Hroot1.
-      {
-        eapply same_root_down0.
-        - apply (@Down_Quantified_inner LindenParameters).
-        - apply Hroot.
-      }
-      specialize (IH Hroot1).
-      rewrite Heqm in IH.
-      specialize (Hrepeat IH).
-      remember (StaticSemantics.countLeftCapturingParensBefore _ ctx) as parenIndex.
-      remember (StaticSemantics.countLeftCapturingParensWithin _ _) as parenCount.
-      assert (def_groups lr = seq (parenIndex + 1) parenCount) as Hgroups_valid by admit.
-      specialize (Hrepeat Hgroups_valid).
-      unfold tMC_valid.
-      intros inp Hinp_compat.
-      unfold tMC_is_tree.
-      intros s Hvalids Hs_inp.
-      specialize (Hrepeat (Semantics.repeatMatcherFuel 0 s)).
-      unfold tm_valid in Hrepeat.
-      specialize (Hrepeat tmc regc cont Htmc_valid).
-      now apply Hrepeat.
-      
-
-    - (* Group *)
-      intros ctx Hroot. simpl.
-      remember (@Group_inner LindenParameters _ :: ctx) as rctx.
-      specialize (IH rctx).
-      assert (Root wroot (wr, rctx)) as Hrootr.
-      {
-        eapply same_root_down0.
-        - subst rctx. apply (@Down_Group_inner LindenParameters).
-        - apply Hroot.
-      }
-      specialize (IH Hrootr).
-      destruct (tCompileSubPattern wr rctx rer forward) as [mr|] eqn:Heqmr; simpl; try exact I.
-      intros tmc regc cont Htmc_tree inp Hinp_compat.
-      unfold tMC_is_tree.
-      intros s Hvalids Hs_inp.
-      remember (fun y: MatchState => _) as tmc2.
-      (* Let's try something *)
-      specialize (IH tmc2 Epsilon (Aclose (S n) :: Areg regc :: cont)).
-      assert (StaticSemantics.countLeftCapturingParensBefore (Group name wr) ctx + 1 = S n) as Heqid by admit.
-      assert (forall inp : input, input_compat inp -> tMC_is_tree tmc2 Epsilon (Aclose (S n) :: Areg regc :: cont) inp) as Htmc2_tree.
-      {
-        intros inp' Hinp'_compat.
-        rewrite Heqtmc2.
-        unfold tMC_is_tree.
-        intros s' Hs'valid Hs'_inp.
-        destruct negb; simpl; try exact I.
-        rewrite Heqid.
-        replace ((S n) =? 0) with false.
-        2: {
-          symmetry.
-          rewrite Nat.eqb_neq.
-          lia.
-        }
-        destruct (List.List.Update.Nat.One.update) as [cap|]; simpl; try exact I.
-        specialize (Htmc_tree inp' Hinp'_compat).
-        unfold tMC_is_tree in Htmc_tree.
-        remember (match_state _ _ cap) as s''.
-        specialize (Htmc_tree s'').
-        assert (Valid (MatchState.input s'') rer s'') as Hs''valid by admit. (* not entirely sure that this is actually true *)
-        specialize (Htmc_tree Hs''valid).
-        assert (ms_matches_inp s'' inp') as Hs''_inp' by admit.
-        specialize (Htmc_tree Hs''_inp').
-        destruct (tmc s'') as [subtree|] eqn:Heqsubtree; simpl; try exact I.
-        apply tree_pop_close.
-        apply tree_pop_reg.
-        assumption.
-      }
+      intros s' Hs'valid Hs'_inp.
+      destruct negb; simpl; try exact I.
       rewrite Heqid.
-      specialize (IH Htmc2_tree inp Hinp_compat).
-      unfold tMC_is_tree in IH.
-      specialize (IH s Hvalids Hs_inp).
-      destruct (mr s tmc2) as [subtree|] eqn:Heqsubtree; simpl; try exact I.
-      apply tree_group.
-      apply is_tree_eps with (cont1 := nil). apply IH.
-  Admitted.
-
-End Main.
+      replace ((S n) =? 0) with false.
+      2: {
+        symmetry.
+        rewrite Nat.eqb_neq.
+        lia.
+      }
+      destruct (List.List.Update.Nat.One.update) as [cap|]; simpl; try exact I.
+      specialize (Htmc_tree inp' Hinp'_compat).
+      unfold tMC_is_tree in Htmc_tree.
+      remember (match_state _ _ cap) as s''.
+      specialize (Htmc_tree s'').
+      assert (Valid (MatchState.input s'') rer s'') as Hs''valid by admit. (* not entirely sure that this is actually true *)
+      specialize (Htmc_tree Hs''valid).
+      assert (ms_matches_inp s'' inp') as Hs''_inp' by admit.
+      specialize (Htmc_tree Hs''_inp').
+      destruct (tmc s'') as [subtree|] eqn:Heqsubtree; simpl; try exact I.
+      apply tree_pop_close.
+      apply tree_pop_reg.
+      assumption.
+    }
+    rewrite Heqid.
+    specialize (IH Htmc2_tree inp Hinp_compat).
+    unfold tMC_is_tree in IH.
+    specialize (IH s Hvalids Hs_inp).
+    destruct (mr s tmc2) as [subtree|] eqn:Heqsubtree; simpl; try exact I.
+    apply tree_group.
+    apply is_tree_eps with (cont1 := nil). apply IH.
+Admitted.
